CollatzFunction/Halt/BStep.lean
@@ -5,12 +5,12 @@ namespace Halt
 
 open Lean Meta Elab Tactic Std Term TmState Γ
 
-lemma B_step (l r: List Γ) (n i: ℕ)
-(h : nth_cfg i = some ⟨B, ⟨one,
+lemma B_step (l r: List Γ) (n i: ℕ) (init_cfg: Cfg)
+(h : nth_cfg init_cfg i = some ⟨B, ⟨one,
   Turing.ListBlank.mk (List.cons zero l),
   Turing.ListBlank.mk (List.replicate (2+n) one ++ zero :: r)⟩⟩)
 :
-nth_cfg (9 + i + n * 2) = some ⟨B, ⟨one,
+nth_cfg init_cfg (9 + i + n * 2) = some ⟨B, ⟨one,
   Turing.ListBlank.mk (zero :: one :: l),
   Turing.ListBlank.mk (List.replicate n one ++ zero :: one :: r)⟩⟩
 := by
@@ -31,12 +31,12 @@ rw [List.replicate_succ] at h
 simp at h
 rw [h]
 
-lemma K_step (l r: List Γ) (n i: ℕ)
-(h : nth_cfg i = some ⟨K, ⟨one,
+lemma K_step (l r: List Γ) (n i: ℕ) (init_cfg)
+(h : nth_cfg init_cfg i = some ⟨K, ⟨one,
   Turing.ListBlank.mk (List.cons zero l),
   Turing.ListBlank.mk (List.replicate (2+n) one ++ zero :: r)⟩⟩)
 :
-nth_cfg (9 + i + n * 2) = some ⟨B, ⟨one,
+nth_cfg init_cfg (9 + i + n * 2) = some ⟨B, ⟨one,
   Turing.ListBlank.mk (zero :: one :: l),
   Turing.ListBlank.mk (List.replicate n one ++ zero :: one :: r)⟩⟩
 := by
