CollatzFunction/Halt/Zeroing.lean
@@ -4,14 +4,14 @@ namespace Halt
 
 open Lean Meta Elab Tactic Std Term TmState
 
-theorem E_zeroing (k : ℕ): ∀ (i : ℕ) (l r : List Γ),
-nth_cfg i = some ⟨E, ⟨Γ.one,
+theorem E_zeroing (k : ℕ): ∀ (i : ℕ) (l r : List Γ) (init_cfg: Cfg),
+nth_cfg init_cfg i = some ⟨E, ⟨Γ.one,
   Turing.ListBlank.mk (List.replicate k Γ.one ++ List.cons Γ.zero l),
   Turing.ListBlank.mk r⟩⟩ →
-nth_cfg (i + k + 1) = some ⟨E, ⟨Γ.zero,
+nth_cfg init_cfg (i + k + 1) = some ⟨E, ⟨Γ.zero,
   Turing.ListBlank.mk l,
   Turing.ListBlank.mk (List.replicate (k+1) Γ.zero ++ r)⟩⟩ := by
-induction k with intros i l r h
+induction k with intros i l r init_cfg h
 | zero => forward h
           ring_nf at *
           simp [h]
